coq/dijkstra_algorithm/priority_queue.v
@@ -1,23 +1,29 @@
-Require Import List ListSet.
+Require Import List ListSet PeanoNat.
+From CAS Require Import 
+  coq.po.from_sg
+  coq.common.compute
+  coq.eqv.properties coq.eqv.structures
+  coq.eqv.theory.
+
+
 Import ListNotations.
 
+
 (* Find a library with proofs *)
-Section Priority_Queue.
+Section Priority_Queue_Def.
 
 
+  Definition Node := nat.
+  
   Context 
-    {A : Type}
-    {Hdec : forall (x y : A), {x = y} + {x <> y}}.
-
-  Context 
-    {U : Type} (* Type *)
-    {C : U -> U -> bool}. (* Comparison operator *)
+    {T : Type} (* Type *)
+    {C : T -> T -> bool}. (* Comparison operator *)
 
 
   (* This function returns the minimum node *)
   Fixpoint find_min_node
-    (ua : U * A)
-    (ls : list (U * A)) : U * A :=
+    (ua : T * Node)
+    (ls : list (T * Node)) : T * Node :=
   match ls with 
   | [] => ua
   | (uy, ay) :: t => 
@@ -30,47 +36,52 @@ Section Priority_Queue.
   end.
 
 
-  (* This theorem asserts that ur is a minimum 
-    element *)
-  Theorem find_min_node_empty_list : 
-    forall ls u a ur ar, 
-    find_min_node (u, a) ls = (ur, ar) ->
-    forall x y, In (x, y) ls -> C ur x = true.
-  Proof.
-    induction ls as [|(uax, uay) ls IHn].
-    + intros ? ? ? ? Ha ? ? Hb.
-      simpl in Ha.
-      inversion Hb.
-    + intros ? ? ? ? Ha ? ? Hb.
-      destruct Hb as [Hb | Hb].
-      inversion Hb;
-      subst; clear Hb.
-      - (* ur is a minimum element *)
-        simpl in Ha.
-  Admitted.
-  (* Why am I trying to prove this? *)    
-
-  
-
 
   Definition remove_min
-    (vs : list A) (* list of nodes *)
-    (f : A -> U) :  (* one row *)
-    option (A * list A) :=
+    (vs : list Node) (* list of nodes *)
+    (f : Node -> T) :  (* one row *)
+    option (Node * list Node) :=
   match vs with 
   | [] => None
   | h :: t => 
     match find_min_node (f h, h) 
       (List.map (fun x => (f x, x)) t) 
     with 
-    | (_, qk) => Some (qk, List.remove Hdec qk vs) 
+    | (_, qk) => Some (qk, List.remove Nat.eq_dec qk vs) 
     end
   end.
+
+End Priority_Queue_Def. (* End of Definitions *)
+  
+Section Priority_Queue_Proofs.
+
+  Context 
+    {T : Type}
+    {zero one : T}
+    {add mul : T -> T -> T}
+    {eqT : brel T}
+    {refT : brel_reflexive T eqT}
+    {symT : brel_symmetric T eqT}
+    {trnT : brel_transitive T eqT}.
+
+
+  (* This theorem asserts that ur is a minimum 
+    element *)
+  Theorem find_min_node_empty_list : 
+    forall ls u a ur ar, 
+    @find_min_node _ (brel_lte_left eqT add) 
+      (u, a) ls = (ur, ar) ->
+    forall x y, In (x, y) ls -> brel_lte_left eqT add ur x = true.
+  Proof.
+  Admitted.
+  
+
   
 
   Lemma remove_min_none_implies_empty_pq : 
-    forall (vs : list A) (f : A -> U),
-    remove_min vs f = None <-> vs = [].
+    forall (vs : list Node) (f : Node -> T),
+    @remove_min _ (brel_lte_left eqT add) vs f = None 
+    <-> vs = [].
   Proof.
     split; intros H.
     + refine(
@@ -82,11 +93,11 @@ Section Priority_Queue.
       end eq_refl).
       rewrite Heq in H.
       simpl in H.
-      destruct (find_min_node (f a, a) 
+      destruct (find_min_node (f n, n) 
       (List.map (fun x => (f x, x)) l));
       inversion H.
     + subst; exact eq_refl.
   Qed.
 
 
-End Priority_Queue
+End Priority_Queue_Proofs.
